dynamic IFC works with z3 4.5.1

examples/rel/DynamicIFC.fst
@@ -1,10 +1,12 @@
 module DynamicIFC
 
 open Rel
-open FStar.DM4F.Heap.IntStoreFixed
-open FStar.DM4F.IntStoreExcFixed
+open Label
+open FStar.DM4F.Heap.LabeledIntStoreFixed
+open FStar.DM4F.LabeledIntStoreExcFixed
 
-module ISFR = FStar.DM4F.IntStoreFixedReader
+module ISFR = FStar.DM4F.LabeledIntStoreFixedReader
+
 
 type binop =
 | Plus
@@ -18,7 +20,7 @@ let interpret_binop o a b =
   | Plus  -> a + b
   | Minus -> a - b
   | Times -> op_Multiply a b
-  | Max   -> if a <= b then b else a
+  | Max   -> if b >= a then b else a
 
 type exp =
 | AInt : int -> exp
@@ -40,56 +42,27 @@ type com =
 | While  : cond:exp -> body:com -> metric:metric -> com
 
 
-(****************************** Preliminaries ******************************)
-
-(* CH: Everything specialized to 2-point lattice *)
-type label =
-| Low
-| High
-
-val op_Less : label -> label -> Tot bool
-let op_Less l1 l2 =
-  match l1, l2 with
-  | Low,High -> true
-  | _, _ -> false
-
-val op_Less_Equals : label -> label -> Tot bool
-let op_Less_Equals l1 l2 =
-  match l1, l2 with
-  | High,Low -> false
-  | _, _ -> true
-
-val join : label -> label -> Tot label
-let join l1 l2 =
-  match l1, l2 with
-  | Low,Low -> Low
-  | _, _ -> High
-
-val meet : label -> label -> Tot label
-let meet l1 l2 =
-  match l1, l2 with
-  | High, High -> High
-  | _, _ -> Low
-
-let universal_property_meet l l1 l2
-  : Lemma (requires (l <= l1 /\ l <= l2)) (ensures (l <= meet l1 l2))
-= ()
-
 type label_fun = id -> Tot label
 
-val update : label_fun -> id -> label -> Tot label_fun
-let update env k v x = if x = k then v else env x
+let trigger_eq (h:rel heap) (x:id) = True
 
-type env_eq (env : rel label_fun) = (forall (x:id). (* {:pattern (env x)} *) (R?.l env) x = (R?.r env) x)
+type env_eq (h : rel heap) = (forall (x:id).  (* {:pattern (trigger_eq h x)} *) snd (sel (R?.l h) x) = snd (sel (R?.r h) x))
 
-type low_equiv (env:label_fun) (h1:rel heap) =
-  (forall (x:id). (* {:pattern (env x)} *) env x = Low ==> index (R?.l h1) x = index (R?.r h1) x)
+type low_equiv (h:rel heap) =
+  (forall (x:id). (* {:pattern (trigger_eq h x)} *) (fun (vl,ll) (vr,lr) -> ll = Low ==> vl = vr)
+      (index (R?.l h) x)  (index (R?.r h) x))
 
-type no_sens_up (env:label_fun) (h:heap) (pc:label) (env':label_fun) (h':heap) =
-  forall (x:id). 
-    (env' x <= env x /\
-    (env x < pc ==> sel h x = sel h' x) /\ 
-    (env x <= pc ==> env x = env' x))
+type low_equiv_env (env:label_fun) (h1:rel heap) =
+  (forall (x:id). env x = Low ==> index (R?.l h1) x = index (R?.r h1) x)
+
+
+type no_sensitive_upd (h:heap) (pc:label) (h':heap) =
+  forall (x:id). (fun (v,l) (v',l') -> 
+    (l' <= l /\
+    (l < pc ==> v = v') /\
+    (l <= pc ==> l = l')))
+      (index h x)  (index h' x)
+
 
 (* TODO : This function is total and does not use exceptions *)
 (* as such it wouldn't be that surprising that writing it in a *)
@@ -100,66 +73,67 @@ type no_sens_up (env:label_fun) (h:heap) (pc:label) (env':label_fun) (h':heap) =
 
 (*  val interpret_exp_st : e:exp -> INT_STORE_EXC int (fun s0 p -> forall opt. p (opt, s0)) *)
 
-let rec interpret_exp_st (e:exp) (env:label_fun) 
+
+let rec interpret_exp_st (e:exp) 
   (* : INT_STORE_EXC int (fun s0 p -> forall x. p (Some x, s0)) *)
   : ISFR.ISRNull (int * label)
 =
   match e with
   | AInt i -> i, Low
-  | AVar x -> ISFR.read x, env x 
+  | AVar x -> ISFR.read x
   | AOp o e1 e2 ->
-    let a,l1 = interpret_exp_st e1 env in
-    let b,l2 = interpret_exp_st e2 env in
+    let a,l1 = interpret_exp_st e1 in
+    let b,l2 = interpret_exp_st e2 in
     interpret_binop o a b, join l1 l2
 
 
 (* unfold *)
-let interpret_exp (h:heap) (e:exp) (env:label_fun) : Tot (int * label) = reify (interpret_exp_st e env) h
+let interpret_exp (h:heap) (e:exp)  : Tot (int * label) = reify (interpret_exp_st e) h
 
 let interpret_exp' (h:heap) (e:exp) : Tot nat =
-  let n,_ = interpret_exp h e (fun _ -> Low) in 
+  let n,_ = interpret_exp h e in
   if 0 > n then 0 else n
 
 (* function used for the decreases clause *)
-val decr_while : heap -> com -> GTot nat 
+val decr_while : heap -> com -> GTot nat
 let decr_while h c =
   match c with
-  | While c b v -> interpret_exp' h v 
+  | While c b v -> interpret_exp' h v
   | _ -> 0
 
 exception OutOfFuel
 exception IfcViolation
 
- val interpret_com_st : c:com -> h0:heap -> env:label_fun -> pc:label -> IntStoreExc label_fun
+ val interpret_com_st : c:com -> h0:heap -> pc:label -> IntStoreExc unit
   (requires (fun h -> h == h0))
   (ensures (fun h _ ho -> h == h0))
   (decreases %[c; decr_while h0 c])
- let rec interpret_com_st c h0 env pc =
+ let rec interpret_com_st c h0 pc =
   match c with
-  | Skip -> env
+  | Skip -> ()
   | Assign x e ->
-    let v, l = interpret_exp_st e env in
-    if  join l pc <= env x then
+    let v, le = interpret_exp_st e in
+    let _, lx = ISFR.read x in 
+    if join le pc <= lx then
     begin
-      write x v; 
-      update env x (join l pc)
+      write x (v, (join le pc))
     end
     else
       raise_  () (* IfcViolation *)
   | Seq c1 c2 ->
     begin
       let h1 = (ISE?.get()) in
-      let env'=  interpret_com_st c1 h1 env pc in 
+      interpret_com_st c1 h1 pc;
       let h2 = (ISE?.get()) in
-      interpret_com_st c2 h2 env' pc
+      interpret_com_st c2 h2 pc
     end
   | If e ct cf ->
-      let v,l  = interpret_exp_st e env in
+      let v,l  = interpret_exp_st e in
       let c = if v = 0 then cf else ct in
       let h = (ISE?.get()) in
-      interpret_com_st c h env (join l pc)
+      interpret_com_st c h (join l pc)
   | While e body v ->
-    let v0, l = interpret_exp_st e env in
+    let v0, l = interpret_exp_st e in
     if v0 <> 0 then
       begin
         (* let m0 = interpret_exp_st v in *)
@@ -171,219 +145,446 @@ exception IfcViolation
         (* interpret_exp_st has that in the spec! *)
         let m0 = interpret_exp' h0 v in
         let h1 = ISE?.get () in
-        let env' = interpret_com_st body h1 env (join l pc) in
+        interpret_com_st body h1 (join l pc);
         let h2 = ISE?.get() in
         let m1 = interpret_exp' h2 v in
         if m0 > m1 then
-          interpret_com_st c h2 env' pc
+          interpret_com_st c h2 pc
         else
           raise_ () (* OutOfFuel *)
       end
-    else
-      env
 
 (* TODO : Normalization does not play very well with ensures clauses... *)
 (* But there is no problem when replacing normalize_term by foobar where *)
 (* abstract let foobar (#a:Type) (x:a) : a = x *)
 (* unfold *)
-let interpret_com (h0:heap) (c:com) (env:label_fun) (pc:label) : Tot (option (label_fun * heap)) 
+let interpret_com (h0:heap) (c:com) (pc:label) : Tot (option heap)
 =
-  match (* normalize_term *) (reify (interpret_com_st c h0 env pc) h0) with
-  | Some env', h -> Some (env', h)
+  match (* normalize_term *) (reify (interpret_com_st c h0 pc) h0) with
+  | Some (), h -> Some h
   | None, _ -> None
 
-(*
-let bidule = assert (reify (interpret_exp_st (AOp Plus (AVar (to_id 7)) (AInt 5))) (create 3) = 8)
-let bidule2 = assert ((interpret_exp (create 3) (AOp Plus (AVar (to_id 7)) (AInt 5))) = 8)
-*)
 
-val dyn_ifc_exp : (e:exp) -> (env:(rel label_fun){env_eq env}) ->
-    (h:(rel heap){low_equiv (R?.l env) h}) -> 
-    Lemma ((fun (vl,ll)  (vr,lr) -> 
-      lr = ll /\ (Low? lr ==> vl = vr)) 
-      (interpret_exp (R?.l h) e (R?.l env))
-      (interpret_exp (R?.r h) e (R?.r env)))
-let rec dyn_ifc_exp e env h  = 
-  match e with 
-  | AInt _ -> ()
-  | AVar _ -> ()
-  | AOp _ e1 e2 -> dyn_ifc_exp e1 env h; dyn_ifc_exp e2 env h
-
-
-val no_sens_trans : (pc:label) -> (pc2:label) -> (env1:label_fun) -> (h1:heap) -> (env2:label_fun) -> (h2:heap) -> (env3:label_fun) -> (h3:heap) ->
+(* Proofs *)
+val no_sens_trans : (pc:label) -> (pc2:label) -> (h1:heap) -> (h2:heap) -> (h3:heap) ->
   Lemma
-    (requires (no_sens_up env1 h1 pc env2 h2 /\ no_sens_up env2 h2 pc2 env3 h3))
-    (ensures (no_sens_up env1 h1 (meet pc pc2) env3 h3))
-let no_sens_trans pc pc2 evn1 h1 env2 h2 env3 h3 = ()
+    (requires (no_sensitive_upd h1 pc h2 /\ no_sensitive_upd h2 pc2 h3))
+    (ensures (no_sensitive_upd h1 (meet pc pc2) h3))
+let no_sens_trans pc pc2 h1 h2 h3 = ()
+
+val no_sens_upd_pc : unit -> 
+  Lemma (forall h h'. no_sensitive_upd h High h' ==> no_sensitive_upd h Low h')
+let no_sens_upd_pc () = () 
+
+type high_pc_type (c:com) (h:heap) (pc:label) = 
+  begin
+    let o = (interpret_com h c pc) in 
+    (Some? o ==> no_sensitive_upd h pc (Some?.v o))
+  end
+
+#set-options "--z3rlimit 10 "
+val high_pc_assign : (x:id) -> (e:exp) -> (h:heap) -> (pc:label) ->
+  Lemma (high_pc_type (Assign x e) h pc)
+let high_pc_assign x e h pc = ()
+#reset-options
 
 
-#set-options "--z3rlimit 500"
-val high_pc : (c:com) -> (env:label_fun) -> (h:heap) -> (pc:label) -> 
+#set-options "--z3rlimit 50 --initial_fuel 1 --max_fuel 1"
+val high_pc_while : (e:exp) -> (body:com) -> (v:exp) -> (h:heap) -> (pc:label) -> 
   Lemma 
-    (requires True)
-    (ensures (fun o -> Some? o ==> (fun (env', h') -> 
-        no_sens_up env h pc env' h'
-      )
-      (Some?.v o))
-      (interpret_com h c env pc))
-  (decreases %[c; decr_while h c])
-let rec high_pc c env h pc = 
-  match c with 
-  | Skip -> () 
-  | Assign x e -> ()
-  | If e ct cf -> 
-      let v0, l = interpret_exp h e env in 
+    (requires 
+      (
+      let c = While e body v in 
+      let v0,l  = interpret_exp h e in
       if v0 <> 0 then
-        high_pc ct env h (join pc l)
-      else
-        high_pc cf env h (join pc l)
-  | Seq c1 c2 -> 
-    let o = interpret_com h c1 env pc in 
-    if Some? o then 
-    begin
-      let env', h' = Some?.v o in 
-      high_pc c1 env h pc;
-      let o2 = interpret_com h' c2 env' pc in 
-      if Some? o2 then 
       begin
-        high_pc c2 env' h' pc;
-        let env'', h'' = Some?.v o2 in 
-        no_sens_trans pc pc env h env' h' env'' h''
+        let o = interpret_com h body (join l pc)in
+        if Some? o then
+        begin
+          let h' = Some?.v o in
+          high_pc_type body h (join l pc) /\
+          begin
+            let m0 = interpret_exp' h v in
+            let m1 = interpret_exp' h' v in
+            if m0 > m1 then
+            begin
+              let o2 = interpret_com h' c pc in
+              if Some? o2 then
+              begin
+                let h'' = Some?.v o2 in
+                high_pc_type c h' pc
+              end
+              else True
+            end
+            else True
+          end
+        end
+        else True
+      end
+      else True))
+    (ensures (high_pc_type (While e body v) h pc))
+let high_pc_while e body v h pc = 
+  let c = While e body v in
+  let r = interpret_com h c pc in
+  let v0,l  = interpret_exp h e in
+  if v0 <> 0 then
+  begin
+    let o = interpret_com h body (join l pc) in
+    if Some? o then
+    begin
+      let h' = Some?.v o in
+      cut (high_pc_type body h (join l pc));
+      let m0 = interpret_exp' h v in
+      let m1 = interpret_exp' h' v in
+      if m0 > m1 then
+      begin
+        let o2 = interpret_com h' c pc in
+        if Some? o2 then
+        begin
+          let h'' = Some?.v o2 in
+          cut (high_pc_type c h' pc);
+          cut (Some? r /\ Some?.v r = h'');
+          no_sens_trans (join l pc) pc h h' h''
+        end
+        else
+          cut(None? r)
+      end
+      else
+        cut(None? r)
+    end
+    else
+      cut(None? r)
+  end
+  else
+    cut (Some? r /\ Some?.v r = h)
+
+#reset-options
+    
+#set-options "--z3rlimit 50 --initial_fuel 1 --max_fuel 1"
+val high_pc : (c:com) -> (h:heap) -> (pc:label) ->
+  Lemma
+    (requires True)
+    (ensures high_pc_type c h pc)
+  (decreases %[c; decr_while h c])
+let rec high_pc c h pc =
+  match c with
+  | Skip -> ()
+  | Assign x e -> high_pc_assign x e h pc
+  | If e ct cf ->
+      let v0, l = interpret_exp h e in
+      if v0 <> 0 then
+        high_pc ct h (join l pc)
+      else
+        high_pc cf h (join l pc);
+      if (Low? pc && High? l) then
+        no_sens_upd_pc ()
+  | Seq c1 c2 -> 
+    let o = interpret_com h c1 pc in
+    if Some? o then
+    begin
+      let h' = Some?.v o in
+      high_pc c1 h pc;
+      let o2 = interpret_com h' c2 pc in
+      if Some? o2 then
+      begin
+        high_pc c2 h' pc;
+        let h'' = Some?.v o2 in
+        no_sens_trans pc pc h h' h''
       end
     end
   | While e body v -> 
-    let v0,l  = interpret_exp h e env in 
+    let v0,l  = interpret_exp h e in
     if v0 <> 0 then
     begin
-      let m0 = interpret_exp' h v in
-      let o = interpret_com h body env (join pc l)in
-      if Some? o then 
+      let o = interpret_com h body (join l pc)in
+      if Some? o then
       begin
-        let env', h' = Some?.v o in 
-        high_pc body env h (join pc l); 
+        let h' = Some?.v o in
+        high_pc body h (join l pc);
+        let m0 = interpret_exp' h v in
         let m1 = interpret_exp' h' v in
         if m0 > m1 then
         begin
-          let o2 = interpret_com h' c env' pc in
-          if Some? o2 then 
+          let o2 = interpret_com h' c pc in
+          if Some? o2 then
           begin
-            let env'', h'' = Some?.v o2 in 
-            high_pc c env' h' pc;
-            no_sens_trans (join pc l) pc env h env' h' env'' h''
+            high_pc c h' pc
           end
         end
       end
-    end
+    end;
+    high_pc_while e body v h pc
 
-#set-options "--z3rlimit 200"
 
-val dyn_ifc : (c:com) -> (env:rel label_fun) -> (pc:label) -> 
-    (h:(rel heap)) -> 
+#reset-options
+
+#set-options "--z3rlimit 15 "
+val dyn_ifc_exp : (e:exp) -> (h:(rel heap)) ->
     Lemma 
-      (requires (low_equiv (R?.l env) h /\ env_eq env))
-      (ensures ((fun r1 r2 -> (Some? r1 /\ Some? r2) ==>  
-        (fun (el,hl) (er,hr) -> 
-          (low_equiv el (R hl hr) /\ 
-           env_eq (R el er) /\
-           no_sens_up  (R?.l env) (R?.l h) pc el hl /\ 
-           no_sens_up  (R?.r env) (R?.r h) pc er hr ))
-        (Some?.v r1) (Some?.v r2))
-      (interpret_com (R?.l h) c (R?.l env) pc)
-      (interpret_com (R?.r h) c (R?.r env) pc)))
-      (decreases %[c; decr_while (R?.l h) c; decr_while (R?.r h) c])
-let rec dyn_ifc c env pc h  = 
-  let (R hl hr) = h in 
-  let (R el er) = env in 
-  high_pc c el hl pc;
-  high_pc c er hr pc;
-  if Low? pc then 
+      (requires (low_equiv h /\ env_eq h))
+      (ensures (
+        let vl,ll = interpret_exp (R?.l h) e in 
+        let vr,lr = interpret_exp (R?.r h) e in 
+          lr = ll /\ (Low? lr ==> vl = vr)))
+let rec dyn_ifc_exp e h  =
+  match e with
+  | AInt _ -> ()
+  | AVar _ -> ()
+  | AOp _ e1 e2 -> dyn_ifc_exp e1 h; dyn_ifc_exp e2 h
+
+
+
+type ifc_type (c:com) (pc:label) (h:rel heap) = 
   begin
-    match c with 
-    | Skip -> ()
-    | Assign x e -> dyn_ifc_exp e env h
-    | If e ct cf ->  
-        dyn_ifc_exp e env h;
-        (match interpret_exp hl e el, interpret_exp hr e er with
-        | (0, ll) , (0, lr) -> 
-            dyn_ifc cf env (join pc ll) h
-        | (0, ll) , (_, lr) -> 
-            cut (High? ll); 
-            high_pc cf el hl High;
-            high_pc ct er hr High; ()
-        | (_, ll) , (0, lr) -> 
-            cut (High? ll); 
-            high_pc ct el hl High;
-            high_pc cf er hr High; ()
-        | (_, ll) , (_, lr) -> 
-            dyn_ifc ct env (join pc ll) h)
-    | Seq c1 c2 -> 
-        let rl = interpret_com hl c1 el pc in 
-        let rr = interpret_com hr c1 er pc in 
-        if (Some? rl && Some? rr) then
+    let ol = (interpret_com (R?.l h) c pc) in 
+     let or = (interpret_com (R?.r h) c pc) in 
+     if (Some? ol && Some? or) then
+     begin
+       let h' = R (Some?.v ol) (Some?.v or) in 
+       low_equiv h' /\ env_eq h'
+     end
+     else True
+  end
+
+
+#set-options "--z3rlimit 30 "
+val dyn_ifc_assign : (x:id) -> (e:exp) -> (pc:label) -> (h:rel heap) -> 
+  Lemma
+      (requires (low_equiv h /\ env_eq h))
+      (ensures (ifc_type (Assign x e) pc h))
+let dyn_ifc_assign x e pc h = dyn_ifc_exp e h 
+#reset-options
+
+
+#set-options "--z3rlimit 50 --initial_fuel 1 --max_fuel 2 "
+val dyn_ifc_while : (e:exp) -> (body:com) -> (v:exp) -> (pc:label) -> (h:rel heap) -> 
+   Lemma
+      (requires (low_equiv h /\ env_eq h /\ 
         begin
-          dyn_ifc c1 env pc h; 
-          let el', hl' = Some?.v rl in 
-          let er', hr' = Some?.v rr in 
-          dyn_ifc c2 (R el' er') pc (R hl' hr')
-        end
-    | While e body v -> 
-      dyn_ifc_exp e env h;
-      let v0l,ll  = interpret_exp hl e el in 
-      let v0r,lr  = interpret_exp hr e er in 
-      (match v0l <> 0, v0r <> 0 with
-      | true, true -> 
-        let ol = interpret_com hl body el (join pc ll)in
-        let or = interpret_com hr body er (join pc lr)in
-        if (Some? ol && Some? or) then
+          let R hl hr = h in 
+          let c = While e body v in 
+          let v0l,ll  = interpret_exp hl e in
+          let v0r,lr  = interpret_exp hr e in
+          match v0l <> 0, v0r <> 0 with
+          | true, true ->  
+            let ol = interpret_com hl body (join ll pc)in
+            let or = interpret_com hr body (join lr pc)in
+            if (Some? ol && Some? or) then
+            begin
+              ifc_type body (join ll pc) h /\ 
+              begin
+                let hl' = Some?.v ol in
+                let hr' = Some?.v or in
+                let m0l = interpret_exp' hl v in
+                let m1l = interpret_exp' hl' v in
+                let m0r = interpret_exp' hr v in
+                let m1r = interpret_exp' hr' v in
+                if m0l > m1l && m0r > m1r then
+                  ifc_type c pc (R hl' hr')
+                else True
+              end
+            end
+            else True
+          | true, false  ->
+            let ol = interpret_com hl body High in
+            if (Some? ol) then
+            begin
+              let hl' = Some?.v ol in
+              let m0l = interpret_exp' hl v in
+              let m1l = interpret_exp' hl' v in
+              if m0l > m1l then
+                ifc_type c pc (R hl' hr)
+              else True
+            end
+            else True
+          | false, true -> 
+            let or = interpret_com hr body High in
+            if (Some? or) then
+            begin
+              let hr' = Some?.v or in
+              let m0r = interpret_exp' hr v in
+              let m1r = interpret_exp' hr' v in
+              if m0r > m1r then
+                ifc_type c pc (R hl hr')
+              else True
+            end
+            else True
+          | false, false -> True
+        end))
+      (ensures (ifc_type (While e body v) pc h))
+let dyn_ifc_while e body v pc h =  
+  let R hl hr = h in 
+  let c = While e body v in 
+  let rl = interpret_com hl c pc in 
+  let rr = interpret_com hr c pc in 
+  let v0l,ll  = interpret_exp hl e in
+  let v0r,lr  = interpret_exp hr e in
+  dyn_ifc_exp e h;
+  match v0l <> 0, v0r <> 0 with
+  | true, true -> 
+      let ol = interpret_com hl body (join ll pc) in
+      let or = interpret_com hr body (join lr pc) in
+      if (Some? ol && Some? or) then
+      begin
         begin
-          dyn_ifc body env (join ll pc) h; 
-          let el', hl' = Some?.v ol in 
-          let er', hr' = Some?.v or in 
-          high_pc body el hl(join ll pc) ;
-          high_pc body er hr(join lr pc) ;
+          cut (ifc_type body (join ll pc) h);
+          let hl' = Some?.v ol in
+          let hr' = Some?.v or in
           let m0l = interpret_exp' hl v in
           let m1l = interpret_exp' hl' v in
           let m0r = interpret_exp' hr v in
           let m1r = interpret_exp' hr' v in
           if m0l > m1l && m0r > m1r then
-            dyn_ifc c (R el' er') pc (R hl' hr')
+          begin
+            cut (ifc_type c pc (R hl' hr'));
+            cut (rl = interpret_com hl' c pc);
+            cut (rr = interpret_com hr' c pc)
+          end
+        end
+      end
+  | true, false ->
+      cut (High? ll);
+      let ol = interpret_com hl body High in
+      if (Some? ol) then
+      begin
+        let hl' = Some?.v ol in
+        high_pc body hl High;
+        let m0l = interpret_exp' hl v in
+        let m1l = interpret_exp' hl' v in
+        if m0l > m1l then
+        begin 
+          cut (ifc_type c  pc (R hl' hr));
+          cut (rl = interpret_com hl' c pc)
+        end
+      end
+  | false, true -> 
+      cut (High? lr);
+      let or = interpret_com hr body High in
+      if (Some? or) then
+      begin
+        let hr' = Some?.v or in
+        high_pc body hr High;
+        let m0r = interpret_exp' hr v in
+        let m1r = interpret_exp' hr' v in
+        if m0r > m1r then
+        begin
+          cut (ifc_type c  pc (R hl hr'));
+          cut (rr = interpret_com hr' c pc)
+        end
+      end
+ | false, false -> ()
+
+#reset-options
+
+
+#set-options "--z3rlimit 50 --initial_fuel 1 --max_fuel 1" 
+val dyn_ifc' : (c:com) -> (pc:label) -> (h:(rel heap)) ->
+    Lemma
+      (requires (low_equiv h /\ env_eq h))
+      (ensures (ifc_type c pc h))
+      (decreases %[c; decr_while (R?.l h) c + decr_while (R?.r h) c])
+let rec dyn_ifc' c pc h  =
+  let (R hl hr) = h in
+  if Low? pc then
+  begin
+    match c with
+    | Skip -> ()
+    | Assign x e -> dyn_ifc_assign x e pc h
+    | If e ct cf ->
+        dyn_ifc_exp e h;
+        (match interpret_exp hl e, interpret_exp hr e with
+        | (0, ll) , (0, lr) ->
+            dyn_ifc' cf (join ll pc) h
+        | (0, ll) , (_, lr) ->
+            cut (High? ll);
+            high_pc cf hl High;
+            high_pc ct hr High 
+        | (_, ll) , (0, lr) ->
+            cut (High? ll);
+            high_pc ct hl High;
+            high_pc cf hr High
+        | (_, ll) , (_, lr) ->
+            dyn_ifc' ct (join ll pc) h)
+    | Seq c1 c2 -> 
+        let ol = interpret_com hl c1 pc in
+        let or = interpret_com hr c1 pc in
+        if (Some? ol && Some? or) then
+        begin
+          dyn_ifc' c1 pc h;
+          let hl' = Some?.v ol in
+          let hr' = Some?.v or in
+          dyn_ifc' c2 pc (R hl' hr')
+        end
+    | While e body v -> 
+      dyn_ifc_exp e h;
+      let v0l,ll  = interpret_exp hl e in
+      let v0r,lr  = interpret_exp hr e in
+      (match v0l <> 0, v0r <> 0 with
+      | true, true ->  
+        let ol = interpret_com hl body (join ll pc)in
+        let or = interpret_com hr body (join lr pc)in
+        if (Some? ol && Some? or) then
+        begin
+          dyn_ifc' body (join ll pc) h;
+          let hl' = Some?.v ol in
+          let hr' = Some?.v or in
+          let m0l = interpret_exp' hl v in
+          let m1l = interpret_exp' hl' v in
+          let m0r = interpret_exp' hr v in
+          let m1r = interpret_exp' hr' v in
+          if m0l > m1l && m0r > m1r then
+            dyn_ifc' c pc (R hl' hr')
         end
       | true, false  ->
-        cut (High? ll);
-        let ol = interpret_com hl body el High in
+        let ol = interpret_com hl body High in
         if (Some? ol) then
         begin
-          let el', hl' = Some?.v ol in 
-          high_pc body el hl High;
+          let hl' = Some?.v ol in
+          high_pc body hl High;
           let m0l = interpret_exp' hl v in
           let m1l = interpret_exp' hl' v in
           if m0l > m1l then
-            dyn_ifc c (R el' er) pc (R hl' hr)
+          begin 
+            dyn_ifc' c  pc (R hl' hr)
+          end
+
         end
       | false, true -> 
-        cut (High? lr);
-        let or = interpret_com hr body er High in
+        let or = interpret_com hr body High in
         if (Some? or) then
         begin
-          let er', hr' = Some?.v or in 
-          high_pc body er hr High;
+          let hr' = Some?.v or in
+          high_pc body hr High;
           let m0r = interpret_exp' hr v in
           let m1r = interpret_exp' hr' v in
           if m0r > m1r then
-            dyn_ifc c (R el er') pc (R hl hr')
+          begin
+            dyn_ifc' c  pc (R hl hr')
+          end
         end
-      | false, false -> ())
+      | false, false -> ());
+      dyn_ifc_while e body v pc h
   end
   else
-    ()
+  begin
+    high_pc c hl pc;
+    high_pc c hr pc
+  end
 
-val dyn_ifc' : (c:com) -> (env:label_fun) -> (pc:label) -> 
-    (h:(rel heap)) -> 
-    Lemma 
-      (requires (low_equiv env h))
-      (ensures ((fun r1 r2 -> (Some? r1 /\ Some? r2) ==>  
-        (fun (el,hl) (er,hr) -> (low_equiv env (R hl hr)))
+#reset-options    
+
+
+val dyn_ifc : (c:com) -> (env:label_fun) -> (pc:label) ->
+    (h:(rel heap)) ->
+    Lemma
+      (requires (low_equiv h /\
+        (forall (x:id). snd (sel (R?.l h) x) = env x /\ 
+                        snd (sel (R?.r h) x) = env x)))
+      (ensures ((fun r1 r2 -> (Some? r1 /\ Some? r2) ==>
+        (fun hl hr -> (low_equiv_env env (R hl hr)))
         (Some?.v r1) (Some?.v r2))
-      (interpret_com (R?.l h) c env pc)
-      (interpret_com (R?.r h) c env pc)))
-let dyn_ifc' c env pc h = dyn_ifc c (R env env) pc h 
+      (interpret_com (R?.l h) c pc)
+      (interpret_com (R?.r h) c pc)))
+let dyn_ifc c env pc h = 
+  dyn_ifc' c pc h; 
+  high_pc c (R?.l h) pc
